theories/MinskyMachines/Reductions/MMA2_to_ndMM2_ACCEPT.v
@@ -13,7 +13,7 @@ From Undecidability.MinskyMachines
   Require Import MMA mma_defs ndMM2.
 
 From Undecidability.Shared.Libs.DLW 
-  Require Import utils Vec.pos Vec.vec Code.sss.
+  Require Import utils Vec.pos Vec.vec Code.subcode Code.sss.
 
 From Undecidability.Synthetic
   Require Import Definitions ReducibilityFacts.
@@ -21,6 +21,9 @@ From Undecidability.Synthetic
 Set Implicit Arguments.
 
 Set Default Proof Using "Type".
+
+Local Tactic Notation "vec2" hyp(v) "into" ident(x) ident(y) :=
+    vec split v with x; vec split v with y; vec nil v; clear v.
 
 Section MMA2_ndMM2.
 
@@ -32,6 +35,11 @@ Section MMA2_ndMM2.
   Notation α := true. 
   Notation β := false.
 
+  Infix "∊" := In (at level 70).
+  Infix "⊆" := incl (at level 70).
+
+  Notation ø := vec_nil.
+
   Definition mma2_instr_enc i (ρ : mm_instr (pos 2)) :=
     match ρ with
       | INCₐ pos0   => INCₙ α i (1+i) :: nil
@@ -40,54 +48,60 @@ Section MMA2_ndMM2.
       | DECₐ _    j => DECₙ β i j :: ZEROₙ β i (1+i) :: nil
     end.
 
+  Notation "'⟨' i , ρ '⟩₁'" := (mma2_instr_enc i  ρ) (format "⟨ i , ρ ⟩₁").
+
+  Reserved Notation "'⟪' i , l '⟫ₗ'" (at level 1, format "⟪ i , l ⟫ₗ").
+
   Fixpoint mma2_linstr_enc i l :=
     match l with
-      | nil => nil
-      | ρ::l => mma2_instr_enc i ρ ++ mma2_linstr_enc (1+i) l
-    end.
+      | nil  => nil
+      | ρ::l => ⟨i,ρ⟩₁ ++ ⟪1+i,l⟫ₗ
+    end
+  where "⟪ i , l ⟫ₗ" := (mma2_linstr_enc i l).
 
-  Fact mma2_linstr_enc_app i l m : mma2_linstr_enc i (l++m) = mma2_linstr_enc i l ++ mma2_linstr_enc (length l+i) m.
+  Fact mma2_linstr_enc_app i l m : ⟪i,l++m⟫ₗ = ⟪i,l⟫ₗ ++ ⟪length l+i,m⟫ₗ.
   Proof.
     revert i; induction l as [ | ? l IHl ]; intros ?; simpl; auto.
     rewrite app_ass, IHl; do 3 f_equal; auto.
   Qed.
 
   Fact mma2_linstr_enc_In i P c : 
-          In c (mma2_linstr_enc i P) 
-       -> exists l r ρ, P = l++ρ::r /\ In c (mma2_instr_enc (length l+i) ρ).
+          c ∊ ⟪i,P⟫ₗ -> exists L ρ R, P = L++ρ::R /\ c ∊ ⟨length L+i,ρ⟩₁.
   Proof.
     revert i; induction P as [ | ρ P IH ]; intros i.
     + intros [].
     + simpl; rewrite in_app_iff; intros [ H | H ].
-      * exists nil, P, ρ; split; auto.
-      * destruct (IH (1+i)) as (l & r & ρ' & H1 & H2); auto.
-        exists (ρ::l), r, ρ'; split; auto.
+      * exists nil, ρ, P; split; auto.
+      * destruct (IH (1+i)) as (l & ρ' & r & H1 & H2); auto.
+        exists (ρ::l), ρ', r; split; auto.
         - simpl; f_equal; auto.
         - eq goal H2; do 2 f_equal; simpl; lia.
   Qed.
 
-  Notation "Σ // a ⊕ b ⊦ u" := (ndmm2_accept Σ a b u) (at level 70, no associativity).
+  Notation "Σ //ₙ a ⊕ b ⊦ u" := (ndmm2_accept Σ a b u) (at level 70, no associativity).
 
-  Notation "i // s -1> t" := (mma_sss i s t).
-  Notation "P // r :1> s" := (sss_step (@mma_sss _) P r s)  (at level 70, no associativity).
-  Notation "P // s ↠ t" := (sss_compute (@mma_sss _) P s t) (at level 70, no associativity).
-  Notation "P // s ~~> t" := (sss_output (@mma_sss _) P s t).
+  Notation "ρ //ₐ s -1> t" := (mma_sss ρ s t) (at level 70, no associativity).
+  Notation "P //ₐ r :1> s" := (sss_step (@mma_sss _) P r s)  (at level 70, no associativity).
+  Notation "P //ₐ s ->> t" := (sss_compute (@mma_sss _) P s t) (at level 70, no associativity).
+  Notation "P //ₐ s ~~> t" := (sss_output (@mma_sss _) P s t) (at level 70, no associativity).
 
-  Local Fact mma2_instr_enc_sound Σ ρ s1 s2 : 
-          ρ // s1 -1> s2 
-       -> match s1, s2 with  
-            | (i,v1), (j,v2) => 
-            let a  := vec_pos v1 pos0 in
-            let b  := vec_pos v1 pos1 in
-            let a' := vec_pos v2 pos0 in
-            let b' := vec_pos v2 pos1 
-            in    incl (mma2_instr_enc i ρ) Σ 
-               -> Σ // a' ⊕ b' ⊦ j 
-               -> Σ // a  ⊕ b  ⊦ i
-          end.
+  Tactic Notation "state" "rebuild" ident(s) hyp(i) hyp(a) hyp(b) :=
+    set (s := (i,a##b##ø));
+    change a with (vec_pos (snd s) pos0);
+    change b with (vec_pos (snd s) pos1);
+    change i with (fst s).
+
+  Local Fact mma2_instr_enc_sound Σ ρ i a b j a' b' : 
+          ρ //ₐ (i,a##b##ø) -1> (j,a'##b'##ø) 
+       -> ⟨i,ρ⟩₁ ⊆ Σ 
+       -> Σ //ₙ a' ⊕ b' ⊦ j 
+       -> Σ //ₙ a  ⊕ b  ⊦ i.
   Proof.
+    state rebuild s1 i a b.
+    state rebuild s2 j a' b'.
+    generalize s1 s2; clear s1 s2 i a b j a' b'.
     induction 1 as [ i x v | i x k v Hv | i x k v u Hv ]; try revert Hv;
-      vec split v with a; vec split v with b; vec nil v; repeat invert pos x; simpl.
+      vec2 v into a b; repeat invert pos x; simpl.
     + constructor 2 with (1+i); auto.
     + constructor 3 with (1+i); auto.
     + intros -> ?; constructor 6 with (1+i); auto.
@@ -96,23 +110,17 @@ Section MMA2_ndMM2.
     + intros -> ?; constructor 5 with k; auto.
   Qed.
 
-  Local Fact mma2_step_linstr_sound Σ P s1 s2 : 
-          (1,P) // s1 :1> s2 
-       -> match s1, s2 with  
-            | (i,v1), (j,v2) => 
-            let a  := vec_pos v1 pos0 in
-            let b  := vec_pos v1 pos1 in
-            let a' := vec_pos v2 pos0 in
-            let b' := vec_pos v2 pos1 
-            in    incl (mma2_linstr_enc 1 P) Σ 
-               -> Σ // a' ⊕ b' ⊦ j 
-               -> Σ // a  ⊕ b  ⊦ i
-          end.
+  Local Fact mma2_step_linstr_sound Σ P i a b j a' b' : 
+          (1,P) //ₐ (i,a##b##ø) :1> (j,a'##b'##ø) 
+       -> ⟪1,P⟫ₗ ⊆  Σ 
+       -> Σ //ₙ a' ⊕ b' ⊦ j 
+       -> Σ //ₙ a  ⊕ b  ⊦ i.
   Proof.
     intros (n & L & ρ & R & v & H1 & H2 & H3).
-    subst s1; destruct s2 as (j,w).
-    inversion H1; subst n P; clear H1; simpl.
-    intros H; apply (mma2_instr_enc_sound _ H3).
+    inversion H1; subst n P; clear H1.
+    inversion H2; subst v i; clear H2.
+    intros H. 
+    apply mma2_instr_enc_sound with (1 := H3).
     apply incl_tran with (2 := H).
     rewrite mma2_linstr_enc_app; simpl.
     rewrite plus_comm.
@@ -121,36 +129,31 @@ Section MMA2_ndMM2.
 
   Variable P : list (mm_instr (pos 2)).
 
-  Definition mma2_prog_enc := STOPₙ 0 :: mma2_linstr_enc 1 P.
+  Definition mma2_prog_enc := STOPₙ 0 :: ⟪1,P⟫ₗ.
   Notation Σ := mma2_prog_enc.
 
-  Local Lemma mma2_prog_enc_compute s1 s2 : 
-          (1,P) // s1 ↠ s2 
-       -> match s1, s2 with  
-            | (i,v1), (j,v2) => 
-            let a  := vec_pos v1 pos0 in
-            let b  := vec_pos v1 pos1 in
-            let a' := vec_pos v2 pos0 in
-            let b' := vec_pos v2 pos1 
-            in    Σ // a' ⊕ b' ⊦ j 
-               -> Σ // a  ⊕ b  ⊦ i
-          end.
+  Local Lemma mma2_prog_enc_sound i a b j a' b'  : 
+          (1,P) //ₐ (i,a##b##ø) ->> (j,a'##b'##ø)
+       -> Σ //ₙ a' ⊕ b' ⊦ j 
+       -> Σ //ₙ a  ⊕ b  ⊦ i.
   Proof.
-    intros (n & Hn).
-    induction Hn as [ (i,v) | n (i,st1) (j,st2) (k,st3) H1 H2 IH2 ]; simpl; auto.
-    revert IH2; simpl; intros IH3 H; generalize (IH3 H).
-    apply (mma2_step_linstr_sound _ H1), incl_tl, incl_refl.
+    intros (n & Hn); revert Hn.
+    state rebuild s1 i a b.
+    state rebuild s2 j a' b'.
+    generalize s1 s2; clear s1 s2 i a b j a' b'.
+    induction 1 as [ (i,v) | n (i,u) (j,v) (k,w) H1 H2 IH2 ]; simpl; auto.
+    revert H1 H2 IH2; vec2 u into au bu; vec2 v into av bv; vec2 w into aw bw.
+    simpl; intros H1 H2 IH3 H; generalize (IH3 H).
+    apply mma2_step_linstr_sound with (1 := H1), incl_tl, incl_refl.
   Qed. 
  
-  Local Lemma mma2_prog_enc_stop : Σ // 0 ⊕ 0 ⊦ 0.
+  Local Lemma mma2_prog_enc_stop : Σ //ₙ 0 ⊕ 0 ⊦ 0.
   Proof. constructor 1; simpl; auto. Qed.
 
   Hint Resolve mma2_prog_enc_stop : core.
 
-  Notation ø := vec_nil.
-
   Local Lemma mma2_prog_enc_complete a b p : 
-             Σ // a ⊕ b ⊦ p -> (1,P) // (p,a##b##ø) ↠ (0,0##0##ø).
+             Σ //ₙ a ⊕ b ⊦ p -> (1,P) //ₐ (p,a##b##ø) ->> (0,0##0##ø).
   Proof.
     induction 1 as [ u H 
                    | a b u v H H1 IH1
@@ -163,12 +166,12 @@ Section MMA2_ndMM2.
       * inversion H; subst u. 
         exists 0; constructor 1.
       * apply mma2_linstr_enc_In in H
-          as (l & r & [ x | x ] & H1 & H2); repeat invert pos x; simpl in H2.
+          as (l & [ x | x ] & r & H1 & H2); repeat invert pos x; simpl in H2.
         1-2: now destruct H2.
         1-2: now destruct H2 as [ | [] ].
     + destruct H as [ H | H ]; try discriminate.
       apply mma2_linstr_enc_In in H
-        as (l & r & [ x | x ] & H3 & H2); repeat invert pos x; simpl in H2.
+        as (l & [ x | x ] & r & H3 & H2); repeat invert pos x; simpl in H2.
       2: now destruct H2.
       2-3: now destruct H2 as [ | [] ].
       destruct H2 as [ H2 | [] ]; inversion H2; subst.
@@ -178,7 +181,7 @@ Section MMA2_ndMM2.
       mma sss stop.
     + destruct H as [ H | H ]; try discriminate.
       apply mma2_linstr_enc_In in H
-        as (l & r & [ x | x ] & H3 & H2); repeat invert pos x; simpl in H2.
+        as (l & [ x | x ] & r & H3 & H2); repeat invert pos x; simpl in H2.
       1: now destruct H2.
       2-3: now destruct H2 as [ | [] ].
       destruct H2 as [ H2 | [] ]; inversion H2; subst.
@@ -188,7 +191,7 @@ Section MMA2_ndMM2.
       mma sss stop.
     + destruct H as [ H | H ]; try discriminate.
       apply mma2_linstr_enc_In in H
-        as (l & r & [ x | x ] & H3 & H2); repeat invert pos x; simpl in H2.
+        as (l & [ x | x ] & r & H3 & H2); repeat invert pos x; simpl in H2.
       1-2: now destruct H2.
       2: now destruct H2 as [ | [] ].
       destruct H2 as [ H2 | H2 ].
@@ -200,7 +203,7 @@ Section MMA2_ndMM2.
       mma sss stop.
     + destruct H as [ H | H ]; try discriminate.
       apply mma2_linstr_enc_In in H
-        as (l & r & [ x | x ] & H3 & H2); repeat invert pos x; simpl in H2.
+        as (l & [ x | x ] & r & H3 & H2); repeat invert pos x; simpl in H2.
       1-2: now destruct H2.
       1: now destruct H2 as [ | [] ].
       destruct H2 as [ H2 | H2 ].
@@ -212,7 +215,7 @@ Section MMA2_ndMM2.
       mma sss stop.
     + destruct H as [ H | H ]; try discriminate.
       apply mma2_linstr_enc_In in H
-        as (l & r & [ x | x j ] & H3 & H2); repeat invert pos x; simpl in H2.
+        as (l & [ x | x j ] & r & H3 & H2); repeat invert pos x; simpl in H2.
       1-2: now destruct H2.
       2: now destruct H2 as [ | [] ].
       destruct H2 as [ H2 | [ H2 | [] ] ].
@@ -224,7 +227,7 @@ Section MMA2_ndMM2.
       mma sss stop.
     + destruct H as [ H | H ]; try discriminate.
       apply mma2_linstr_enc_In in H
-        as (l & r & [ x | x j ] & H3 & H2); repeat invert pos x; simpl in H2.
+        as (l & [ x | x j ] & r & H3 & H2); repeat invert pos x; simpl in H2.
       1-2: now destruct H2.
       1: now destruct H2 as [ | [] ].
       destruct H2 as [ H2 | [ H2 | [] ] ].
@@ -236,14 +239,14 @@ Section MMA2_ndMM2.
       mma sss stop.
   Qed.
 
-  Theorem MMA2_ndMM2_equiv a b : MMA2_HALTS_ON_ZERO (P,a##b##ø) <-> Σ // a ⊕ b ⊦ 1.
+  Theorem MMA2_ndMM2_equiv a b : (1,P) //ₐ (1,a##b##ø) ~~> (0,0##0##ø) 
+                             <-> Σ //ₙ a ⊕ b ⊦ 1.
   Proof.
     split.
     + intros (H1 & _). 
-      apply mma2_prog_enc_compute in H1.
-      apply H1; auto.
-    + intros H1; split.
-      * apply mma2_prog_enc_complete, H1.
+      now apply mma2_prog_enc_sound with (1 := H1).
+    + split.
+      * now apply mma2_prog_enc_complete.
       * simpl; lia.
   Qed.
 
@@ -252,8 +255,7 @@ End MMA2_ndMM2.
 Theorem reduction : MMA2_HALTS_ON_ZERO ⪯ @ndMM2_ACCEPT nat.
 Proof.
   apply reduces_dependent; exists.
-  intros (P & v). 
-  vec split v with a; vec split v with b; vec nil v.
+  intros (P & v); vec2 v into a b. 
   exists (existT _ (mma2_prog_enc P) (1,(a,b))).
   apply MMA2_ndMM2_equiv.
 Qed.
